src/program_proof/util_proof.v
@@ -96,4 +96,27 @@ Proof.
   apply bool_decide_iff, sum_overflow_check.
 Qed.
 
+Theorem wp_CloneByteSlice stk E s q vs :
+  {{{ is_slice_small s u8T q vs }}}
+    CloneByteSlice (slice_val s) @ stk; E
+  {{{ (s':Slice.t), RET (slice_val s'); is_slice_small s u8T q vs ∗ is_slice s' u8T 1 vs }}}.
+Proof.
+  iIntros (Φ) "Hs HΦ".
+  wp_call.
+  wp_apply wp_slice_len.
+  iDestruct (is_slice_small_sz with "Hs") as %Hlen.
+  wp_apply wp_new_slice; first by auto.
+  iIntros (s') "Hs'".
+  iDestruct (is_slice_small_acc with "Hs'") as "[Hs'_small Hs']".
+  wp_pures.
+  wp_apply (wp_SliceCopy_full with "[$Hs $Hs'_small]").
+  { iPureIntro.
+    autorewrite with len.
+    auto. }
+  iIntros "(Hs&Hs'_small)".
+  iSpecialize ("Hs'" with "Hs'_small").
+  wp_pures.
+  iApply ("HΦ" with "[$]").
+Qed.
+
 End heap.
